GoLean/GoCore.lean
@@ -1,3 +1,4 @@
 import GoLean.GoCore.Machine
+import GoLean.GoCore.StateWf
 import GoLean.GoCore.StepFn
 import GoLean.GoCore.MachineSound
